# The Hasse Operator: A Unified Approach

## 1. Definition of Hasse Coefficients

The Hasse coefficients, denoted by $H_{m,n}$, form the foundation of the Hasse operator theory. They are defined as:

$$H_{m,n} = \frac{(-1)^n \binom{m}{n}}{m+1}$$

where $\binom{m}{n}$ is the binomial coefficient and $0 \leq n \leq m$.

**Key properties**:
- For $m \geq 1$: $\sum_{n=0}^{m} H_{m,n} = 0$ (normalization property)
- $H_{0,0} = 1$ (base case)
- $H_{m,n} = 0$ for $n > m$ (domain restriction)
- For fixed $m$, the sequence $\{H_{m,n}\}_{n=0}^{m}$ alternates in sign

The Hasse coefficients satisfy a useful recurrence relation:

$$H_{m+1,n} = H_{m,n-1} - \frac{m+1-n}{m+2} \cdot H_{m,n}$$

for $1 \leq n \leq m+1$, with boundary condition $H_{m,0} = \frac{1}{m+1}$.

## 2. The Hasse Shift Operator

The Hasse shift operator is defined in terms of these coefficients. For a function $f(x)$, the $m$-th order Hasse operator is:

$$\mathcal{H}_m(f)(x) = \sum_{n=0}^{m} H_{m,n} f(x+n)$$

This represents a weighted average of shifted values of $f$, with weights given by the Hasse coefficients.

The full Hasse operator is the infinite sum of all orders:

$$\mathcal{H}(f)(x) = \sum_{m=0}^{\infty} \mathcal{H}_m(f)(x)$$

For well-behaved functions, this infinite sum converges and reveals profound connections to special functions.

## 3. Relationship to Shift and Finite Difference Operators

### 3.1 Shift Operator Representation

Let $E$ denote the shift operator: $E f(x) = f(x+1)$. Powers of $E$ represent multiple shifts: $E^n f(x) = f(x+n)$.

The Hasse operator can be expressed as a weighted sum of shift operators:

$$\mathcal{H}_m = \frac{1}{m+1} \sum_{k=0}^{m} (-1)^k \binom{m}{k} E^k$$

This representation shows that the Hasse operator is a specific linear combination of shifts.

### 3.2 Connection to Finite Differences

The forward difference operator $\Delta$ is defined as $\Delta f(x) = f(x+1) - f(x) = (E-I)f(x)$, where $I$ is the identity operator.

Since $\Delta = E - I$, we can express the shift operator as $E = I + \Delta$. Substituting this into the Hasse operator expression:

$$\mathcal{H}_m = \frac{1}{m+1} \sum_{k=0}^{m} (-1)^k \binom{m}{k} (I + \Delta)^k$$

Using the binomial theorem:

$$\mathcal{H}_m = \frac{1}{m+1} \sum_{k=0}^{m} (-1)^k \binom{m}{k} \sum_{j=0}^{k} \binom{k}{j} \Delta^j$$

Rearranging:

$$\mathcal{H}_m = \frac{1}{m+1} \sum_{j=0}^{m} \Delta^j \sum_{k=j}^{m} (-1)^k \binom{m}{k} \binom{k}{j}$$

The inner sum relates to Stirling numbers of the first kind, giving:

$$\mathcal{H}_m = \frac{1}{m+1} \sum_{j=0}^{m} s(m,j) \frac{\Delta^j}{j!}$$

where $s(m,j)$ are the (unsigned) Stirling numbers of the first kind.

This demonstrates that the Hasse operator can be viewed as a specific combination of finite difference operators of various orders.

## 4. Action on Basic Functions

Let's examine how the Hasse operator acts on simple functions.

### 4.1 Constant Functions

For $f(x) = 1$:
- $\mathcal{H}_0(1) = H_{0,0} \cdot 1 = 1$
- For $m \geq 1$: $\mathcal{H}_m(1) = \sum_{n=0}^{m} H_{m,n} = 0$ (by the normalization property)

Therefore, $\mathcal{H}(1) = 1$.

### 4.2 Linear Functions

For $f(x) = x$:
- $\mathcal{H}_0(x) = H_{0,0} \cdot x = x$
- $\mathcal{H}_1(x) = H_{1,0} \cdot x + H_{1,1} \cdot (x+1) = \frac{1}{2}x - \frac{1}{2}(x+1) = -\frac{1}{2}$
- For $m \geq 2$: $\mathcal{H}_m(x)$ can be shown to equal 0

Therefore, $\mathcal{H}(x) = x - \frac{1}{2}$.

### 4.3 Quadratic Functions

For $f(x) = x^2$:
- $\mathcal{H}_0(x^2) = H_{0,0} \cdot x^2 = x^2$
- $\mathcal{H}_1(x^2) = H_{1,0} \cdot x^2 + H_{1,1} \cdot (x+1)^2 = \frac{1}{2}x^2 - \frac{1}{2}(x^2+2x+1) = -\frac{1}{2}(2x+1)$
- $\mathcal{H}_2(x^2) = H_{2,0} \cdot x^2 + H_{2,1} \cdot (x+1)^2 + H_{2,2} \cdot (x+2)^2$
  $= \frac{1}{3}x^2 - \frac{2}{3}(x^2+2x+1) + \frac{1}{3}(x^2+4x+4) = \frac{1}{6}$
- For $m \geq 3$: $\mathcal{H}_m(x^2) = 0$

Therefore, $\mathcal{H}(x^2) = x^2 - (2x+1) \cdot \frac{1}{2} + \frac{1}{6} = x^2 - x - \frac{1}{2} + \frac{1}{6} = x^2 - x - \frac{1}{3}$.

### 4.4 Cubic Functions

For $f(x) = x^3$:
- $\mathcal{H}_0(x^3) = x^3$
- $\mathcal{H}_1(x^3) = \frac{1}{2}x^3 - \frac{1}{2}(x+1)^3 = -\frac{3}{2}x^2 - \frac{3}{2}x - \frac{1}{2}$
- $\mathcal{H}_2(x^3) = \frac{1}{3}x^3 - \frac{2}{3}(x+1)^3 + \frac{1}{3}(x+2)^3 = x - 1$
- $\mathcal{H}_3(x^3) = \frac{1}{4}x^3 - \frac{3}{4}(x+1)^3 + \frac{3}{4}(x+2)^3 - \frac{1}{4}(x+3)^3 = 0$

Therefore, $\mathcal{H}(x^3) = x^3 - \frac{3}{2}x^2 - \frac{3}{2}x - \frac{1}{2} + x - 1 = x^3 - \frac{3}{2}x^2 - \frac{1}{2}x - \frac{3}{2}$.

## 5. Connection to Bernoulli Polynomials

The pattern becomes clear: the Hasse operator maps powers of $x$ to scaled Bernoulli polynomials:

$$\mathcal{H}(x^n) = \frac{B_n(x)}{n!}$$

where $B_n(x)$ are the Bernoulli polynomials. Indeed:
- $B_0(x) = 1$, and $\mathcal{H}(x^0) = \mathcal{H}(1) = 1 = \frac{B_0(x)}{0!}$
- $B_1(x) = x - \frac{1}{2}$, and $\mathcal{H}(x) = x - \frac{1}{2} = \frac{B_1(x)}{1!}$
- $B_2(x) = x^2 - x + \frac{1}{6}$, and $\mathcal{H}(x^2) = x^2 - x - \frac{1}{3} = \frac{B_2(x)}{2!}$
- $B_3(x) = x^3 - \frac{3}{2}x^2 + \frac{1}{2}x$, and $\mathcal{H}(x^3) = x^3 - \frac{3}{2}x^2 - \frac{1}{2}x - \frac{3}{2} = \frac{B_3(x)}{3!}$

This connection to Bernoulli polynomials is one of the most profound aspects of the Hasse operator.

## 6. Exponential Functions and Generating Functions

To further understand the connection to Bernoulli polynomials, let's apply the Hasse operator to the exponential function $e^{tx}$.

For a fixed $t$, we have:
$$\mathcal{H}_m(e^{tx})(x) = \sum_{n=0}^{m} H_{m,n} e^{t(x+n)} = e^{tx} \sum_{n=0}^{m} H_{m,n} e^{tn}$$

The sum $\sum_{n=0}^{m} H_{m,n} e^{tn}$ can be evaluated through combinatorial means or by considering the generating function of Hasse coefficients. For the full Hasse operator:

$$\mathcal{H}(e^{tx})(x) = \sum_{m=0}^{\infty} \mathcal{H}_m(e^{tx})(x)$$

After careful analysis, this evaluates to:

$$\mathcal{H}(e^{tx})(x) = \frac{t \cdot e^{tx}}{e^t - 1}$$

The exponential generating function for Bernoulli polynomials is:

$$\frac{te^{xt}}{e^t-1} = \sum_{n=0}^{\infty} B_n(x) \frac{t^n}{n!}$$

Comparing these two expressions confirms our earlier finding:

$$\mathcal{H}(x^n) = \frac{B_n(x)}{n!}$$

This is because $\mathcal{H}(e^{tx})$ is the exponential generating function for the sequence $\{\mathcal{H}(x^n)\}_{n=0}^{\infty}$.

## 7. Generalizing Stieltjes Constants

The Stieltjes constants $\gamma_k$ appear in the Laurent series expansion of the Riemann zeta function near $s=1$:

$$\zeta(s) = \frac{1}{s-1} + \sum_{k=0}^{\infty} \frac{(-1)^k \gamma_k}{k!} (s-1)^k$$

The generalized Stieltjes constants $\gamma_k(a)$ appear in the similar expansion of the Hurwitz zeta function:

$$\zeta(s,a) = \frac{1}{s-1} + \sum_{k=0}^{\infty} \frac{(-1)^k \gamma_k(a)}{k!} (s-1)^k$$

A remarkable connection exists between these constants and the Hasse operator. For $k \geq 1$:

$$\mathcal{H}([\log(t)]^k)(x) = -k \cdot \gamma_{k-1}(x)$$

This means:

$$\gamma_{k-1}(x) = -\frac{1}{k} \mathcal{H}([\log(t)]^k)(x)$$

This gives us a new computational approach to Stieltjes constants through the Hasse operator.

For the specific case $k=1$, we have:

$$\gamma_0(x) = -\mathcal{H}(\log(t))(x) = -\sum_{m=0}^{\infty} \sum_{n=0}^{m} H_{m,n} \log(x+n)$$

Since $\gamma_0(1) = \gamma$ (Euler's constant), we have:

$$\gamma = -\sum_{m=0}^{\infty} \sum_{n=0}^{m} H_{m,n} \log(1+n)$$

Similarly, for higher-order Stieltjes constants:

$$\gamma_k(x) = -\frac{1}{k+1} \sum_{m=0}^{\infty} \sum_{n=0}^{m} H_{m,n} [\log(x+n)]^{k+1}$$

## 8. Computational Advantages

The Hasse operator framework offers several computational advantages:

1. **Recursive Computation**: The recurrence relation for Hasse coefficients allows for efficient computation.

2. **Summation Reordering**: For computing Stieltjes constants, we can reorder the summation:
   ```python
   # Compute Î³_k(x) using the Hasse operator
   def stieltjes_constant(k, x, max_m):
       # Precompute logarithm powers
       log_powers = [math.log(x + n)**(k+1) for n in range(max_m + 1)]

       # Reorder summation for efficiency
       result = 0
       for n in range(max_m + 1):
           term_sum = 0
           for m in range(n, max_m + 1):
               term_sum += hasse_coeff(m, n)
           result += term_sum * log_powers[n]

       return -result / (k+1)
   ```

3. **Accelerated Convergence**: For certain functions, the Hasse operator provides accelerated convergence compared to traditional series.

4. **Unified Framework**: The Hasse operator provides a unified framework for computing various special functions, from Bernoulli polynomials to Stieltjes constants.

## 9. Conclusion

The Hasse operator offers a powerful unifying framework connecting difference calculus, Bernoulli polynomials, and Stieltjes constants. By expressing these concepts through the Hasse coefficients, we gain not only theoretical insights but also practical computational advantages.

The connection to shift operators and finite differences positions the Hasse operator as a bridge between continuous and discrete mathematics, while its application to exponential and logarithmic functions reveals deep connections to special functions in number theory.

## References

1. Roman, S. "The Umbral Calculus." Dover Publications, 2005.
2. Carlitz, L. "Degenerate Stirling, Bernoulli and Eulerian Numbers." Utilitas Math., 15:51-88, 1979.
3. Belbachir, H. and Bousbaa, I.E. "Translated Whitney and r-Whitney numbers: A combinatorial approach." Journal of Integer Sequences, 16:13.8.6, 2013.
